src/complete_poset.lean
@@ -1,0 +1,99 @@
+/-
+Copyright (c) 2022 Markus Himmel. All rights reserved.
+Released under Apache 2.0 license as described in the file LICENSE.
+Authors: Markus Himmel
+-/
+import tactic
+import order.hom.basic
+import data.set.lattice
+
+universes u v
+
+variables {α : Type u} {β : Type v}
+
+namespace my
+
+section
+variables [partial_order α]
+
+@[ext] class has_supremum (S : set α) :=
+(supremum : α)
+(upper_bound : ∀ x ∈ S, x ≤ supremum)
+(least_upper_bound : ∀ (y : α), (∀ x ∈ S, x ≤ y) → supremum ≤ y)
+
+def _root_.set.supremum (S : set α) [has_supremum S] : α :=
+has_supremum.supremum S
+
+lemma le_supremum (S : set α) [has_supremum S] {x : α} (hx : x ∈ S) : x ≤ S.supremum :=
+has_supremum.upper_bound _ hx
+
+lemma supremum_le (S : set α) [has_supremum S] {y : α} (hy : ∀ x ∈ S, x ≤ y) : S.supremum ≤ y :=
+has_supremum.least_upper_bound _ hy
+
+instance (S : set α) : subsingleton (has_supremum S) :=
+⟨λ s₁ s₂, has_supremum.ext _ _ (le_antisymm
+  (@has_supremum.least_upper_bound _ _ _ s₁ _ $ @has_supremum.upper_bound _ _ _ s₂)
+  (@has_supremum.least_upper_bound _ _ _ s₂ _ $ @has_supremum.upper_bound _ _ _ s₁))⟩
+
+end
+
+class complete_partial_order (α : Type u) extends partial_order α :=
+(has_supremum : ∀ (S : set α), has_supremum S)
+
+instance complete_partial_order_has_supremum [complete_partial_order α] (S : set α) : has_supremum S :=
+complete_partial_order.has_supremum _
+
+instance : complete_partial_order (set α) :=
+{ has_supremum := λ S,
+  { supremum := ⋃₀ S,
+    upper_bound := λ T, set.subset_sUnion_of_mem,
+    least_upper_bound := λ T hT x ⟨y, ⟨hy, hy'⟩⟩, hT _ hy hy' },
+  ..(infer_instance : partial_order (set α)) }
+
+theorem knaster_tarski [complete_partial_order α] (f : α → α) (hf : monotone f) : ∃ x, f x = x :=
+let s := {x | x ≤ f x}.supremum in
+have s ≤ f s, from supremum_le _ $ λ x hx, le_trans hx $ hf $ le_supremum _ hx,
+⟨s, le_antisymm (le_supremum _ $ hf this) this⟩
+
+theorem cantor_schroeder_bernstein (f : α → β) (hf : function.injective f) (g : β → α) (hg : function.injective g) :
+  nonempty (α ≃ β) :=
+begin
+  by_cases hβ : nonempty β,
+  { haveI hα : nonempty α := nonempty.map g hβ,
+    have h : monotone (compl ∘ set.image g ∘ compl ∘ set.image f),
+    { exact (compl_antitone _).comp (set.monotone_image.comp_antitone ((compl_antitone _).comp_monotone set.monotone_image)) },
+    obtain ⟨P, hP : (g '' (f '' P)ᶜ)ᶜ = P⟩ := knaster_tarski _ h,
+    classical,
+    refine ⟨equiv.of_bijective (P.piecewise f (function.inv_fun g)) ⟨λ x y hxy, _, _⟩⟩,
+    { by_cases hx : x ∈ P,
+      { rw [set.piecewise_eq_of_mem _ _ _ hx] at hxy,
+        have : y ∈ P,
+        { rw [←hP],
+          rintro ⟨z, ⟨hz, rfl⟩⟩,
+          refine hz ⟨x, ⟨hx, _⟩⟩,
+          have : g z ∉ P,
+          { rw [←hP, set.mem_compl_iff, not_not],
+            exact set.mem_image_of_mem _ hz },
+          rw [hxy, set.piecewise_eq_of_not_mem _ _ _ this, function.left_inverse_inv_fun hg] },
+        rw [set.piecewise_eq_of_mem _ _ _ this] at hxy,
+        exact hf hxy },
+      { rw [set.piecewise_eq_of_not_mem _ _ _ hx] at hxy,
+        rw [←hP, set.mem_compl_iff, not_not] at hx,
+        rcases hx with ⟨z, ⟨hz, rfl⟩⟩,
+        rw [function.left_inverse_inv_fun hg] at hxy,
+        have hyP : y ∉ P,
+        { refine λ hy, hz ⟨y, ⟨hy, _⟩⟩,
+          rw [hxy, set.piecewise_eq_of_mem _ _ _ hy] },
+        have := hyP,
+        rw [←hP, set.mem_compl_iff, not_not] at this,
+        rcases this with ⟨w, ⟨hw, rfl⟩⟩,
+        rw [hxy, set.piecewise_eq_of_not_mem _ _ _ hyP, function.left_inverse_inv_fun hg] } },
+    { simp only [←set.range_iff_surjective, set.range_piecewise, set.eq_univ_iff_forall, set.mem_union, or_iff_not_imp_left],
+      refine λ x hx, ⟨g x, ⟨_, function.left_inverse_inv_fun hg _⟩⟩,
+      rw [←hP, compl_compl],
+      exact set.mem_image_of_mem _ hx } },
+  { haveI := not_nonempty_iff.1 hβ,
+    refine ⟨⟨f, g, λ x, false.elim (is_empty.false (f x)), λ x, false.elim (is_empty.false x)⟩⟩ }
+end
+
+end my
