src/predicate_logic.lean
@@ -1,0 +1,61 @@
+/-
+Copyright (c) 2022 Markus Himmel. All rights reserved.
+Released under Apache 2.0 license as described in the file LICENSE.
+Authors: Markus Himmel
+-/
+import tactic
+
+open_locale classical
+noncomputable theory
+
+section
+
+structure context :=
+(var function relation : Type*)
+(fun_arity : function → ℕ)
+(rel_arity : relation → ℕ)
+
+open context
+
+variable (C : context)
+
+inductive term
+| tvar (i : var C) : term
+| app (f : function C) (arg : fin (fun_arity C f) → term) : term
+
+inductive formula
+| false : formula
+| fterm : term C → formula
+| eq : term C → term C → formula
+| rel (φ : relation C) : (fin (rel_arity C φ) → term C) → formula
+| imp : formula → formula → formula
+| uni : var C → formula → formula
+
+instance : has_bot (formula C) := ⟨formula.false⟩
+local infix ⇒:80 := formula.imp
+local notation `¬'`:90 p:90 := p ⇒ ⊥
+instance : has_coe (term C) (formula C) := ⟨formula.fterm⟩
+local infix `='`:50 := formula.eq
+local notation `∀'`:40 x:40 `: `:40 p:40 := formula.uni x p
+
+end
+
+open context
+
+namespace term
+variables {C : context}
+
+noncomputable def subst (x : var C) (t : term C) : term C → term C
+| (tvar i) := if i = x then t else tvar i
+| (app f arg) := app f (subst ∘ arg)
+
+end term
+
+namespace formula
+variables {C : context}
+
+def subst (x : var C) (t : term C) : formula C → formula C
+| false := false
+| (fterm t) := fterm t
+
+end formula
